tests/ssrpattern.v
@@ -1,9 +1,4 @@
-Require Import ssrmatching.ssrmatching.
-
-Require Import Mtac2.Mtac2.
-
-Ltac ssrpattern p := ssrpattern p.
-Definition ssrpattern {A} (x:A) := T.ltac "ssrpattern" [m: Dyn x].
+From Mtac2 Require Import Mtac2.
 
 Goal (3+5, 0) = (10, 0).
 MProof.
@@ -14,4 +9,17 @@ MProof.
   e <- M.evar nat;
   f <- M.evar nat;
   ssrpattern (e+f);; (mif M.is_evar e then T.ret tt else M.failwith "evar instantiated"): tactic.
+Abort.
+
+Import M.notations.
+(* abstract _from_sort and _from_term *)
+Goal True->True.
+MProof.
+  f <- abstract_from_sort (s:=Sorts.Sorts.SProp) 3 (3+3 = 6);
+  M.print_term f;;
+  M.ret _.
+Unshelve.
+  f <- abstract_from_term 3 (_+3 = 6);
+  M.print_term f;;
+  M.ret _.
 Abort.
